Lp2lc/Active/STLC/__Infer_umbral.lean
@@ -7,10 +7,10 @@ open Lp2lc.Active.Util
 namespace Umbral
 
 -- TODO: enable it
--- structure TypeWithSafey [build : BuildEnv]
---     (trm : AST.Trm build.ExeParameters) where
+-- structure TypeWithSafey [core : EnvCore] [build : BuildEnv core]
+--     (trm : AST.Trm core.ExeParameters) where
 --   t2 : AST.Typ build.BuildParameters
---   safety : [exe : CompatExeEnv build] -> Safety trm t2
+--   safety : [exe : ExeEnv core] -> Safety trm t2
 
 /-
 TODO: discharge this function.
@@ -19,9 +19,9 @@ In general function should have identical structure with Trm.infer in __Infer.le
 
 The original trm2valCtx and trm2typCtx are not designed to hold TypeWithSafey, you will need to make some new context for that
 -/
-/-- Infers build types for executable terms. -/
-def infer [build : BuildEnv] [env : CompatExeEnv build]
-    (trm : AST.Trm env.ExeParameters) : RecOpt (TypeWithSafey trm) := sorry
+-- /-- Infers build types for executable terms. -/
+-- def infer [core : EnvCore] [build : BuildEnv core] [env : ExeEnv core]
+--     (trm : AST.Trm core.ExeParameters) : RecOpt (TypeWithSafey trm) := sorry
 
 end Umbral
 
